Earley impl draft.

Earley.thy
@@ -2,7 +2,7 @@ theory Earley
   imports 
     LocalLexing.CFG
     LocalLexing.Derivations
-    LocalLexing.LLEarleyParsing \<comment>\<open>TODO: Rewrite\<close>
+    LocalLexing.LLEarleyParsing \<comment>\<open>Rewritten\<close>
     LocalLexing.Validity \<comment>\<open>TODO: Rewrite\<close>
     LocalLexing.TheoremD2 \<comment>\<open>TODO: Rewrite\<close>
     LocalLexing.TheoremD4 \<comment>\<open>TODO: Rewrite\<close>
@@ -35,7 +35,13 @@ lemma (in CFG) is_word_simp:
 
 section \<open>Earley Parsing Algorithm\<close>
 
-subsection \<open>Earley Items, Bin, Bins, State\<close>
+subsection \<open>Earley Items, Bin(s), State\<close>
+
+definition rule_head :: "rule \<Rightarrow> symbol" where
+  "rule_head = fst"
+
+definition rule_body :: "rule \<Rightarrow> symbol list" where
+  "rule_body = snd"
 
 datatype item = 
   Item 
@@ -45,29 +51,29 @@ datatype item =
 
 type_synonym items = "item set"
 
-definition item_nonterminal :: "item \<Rightarrow> symbol" where
-  "item_nonterminal x = fst (item_rule x)"
+definition item_rule_head :: "item \<Rightarrow> symbol" where
+  "item_rule_head x = rule_head (item_rule x)"
 
-definition item_rhs :: "item \<Rightarrow> sentence" where
-  "item_rhs x = snd (item_rule x)"
+definition item_rule_body :: "item \<Rightarrow> sentence" where
+  "item_rule_body x = rule_body (item_rule x)"
 
 definition item_\<alpha> :: "item \<Rightarrow> sentence" where
-  "item_\<alpha> x = take (item_dot x) (item_rhs x)"
+  "item_\<alpha> x = take (item_dot x) (item_rule_body x)"
 
 definition item_\<beta> :: "item \<Rightarrow> sentence" where 
-  "item_\<beta> x = drop (item_dot x) (item_rhs x)"
+  "item_\<beta> x = drop (item_dot x) (item_rule_body x)"
 
 definition init_item :: "rule \<Rightarrow> nat \<Rightarrow> item" where
   "init_item r k = Item r 0 k"
 
 definition is_complete :: "item \<Rightarrow> bool" where
-  "is_complete x = (item_dot x \<ge> length (item_rhs x))"
+  "is_complete x = (item_dot x \<ge> length (item_rule_body x))"
 
 definition (in CFG) is_finished :: "item \<Rightarrow> bool" where
-  "is_finished x = (item_nonterminal x = \<SS> \<and> item_origin x = 0 \<and> is_complete x)"
+  "is_finished x = (item_rule_head x = \<SS> \<and> item_origin x = 0 \<and> is_complete x)"
 
 definition next_symbol :: "item \<Rightarrow> symbol option" where
-  "next_symbol x = (if is_complete x then None else Some ((item_rhs x) ! (item_dot x)))"
+  "next_symbol x = (if is_complete x then None else Some ((item_rule_body x) ! (item_dot x)))"
 
 definition inc_item :: "item \<Rightarrow> item" where
   "inc_item x = Item (item_rule x) (item_dot x + 1) (item_origin x)"
@@ -91,8 +97,16 @@ definition is_finished_bin :: "state \<Rightarrow> bool" where
 definition current_item :: "state \<Rightarrow> item" where
   "current_item s = ((bins s)!(bin s))!index s"
 
+fun contains :: "('a \<Rightarrow> bool) \<Rightarrow> 'a list \<Rightarrow> bool" where
+  "contains _ [] \<longleftrightarrow> False"
+| "contains f (x#xs) \<longleftrightarrow> (if f x then True else contains f xs)"
+  
 definition update_bins :: "bins \<Rightarrow> nat \<Rightarrow> item list \<Rightarrow> bins" where
-  "update_bins bs k is = (bs[k := bs!k @ is])"
+  "update_bins bs k is = (
+    let bin = bs!k in
+    let is = filter (\<lambda>i. \<not> contains (\<lambda>j. i = j) bin) is in
+    (bs[k := bin @ is])
+  )"
 
 subsection \<open>Earley Algorithm\<close>
 
@@ -103,7 +117,7 @@ locale Earley = CFG +
   assumes valid_rules: "set rules = \<RR> \<and> distinct rules"
 begin
 
-definition earley_step :: "state \<Rightarrow> state" where \<comment>\<open>TODO\<close>
+definition earley_step :: "state \<Rightarrow> state" where
   "earley_step s = (
     if is_finished_state s then
       s
@@ -113,13 +127,20 @@ definition earley_step :: "state \<Rightarrow> state" where \<comment>\<open>TOD
       let item = current_item s in
       case next_symbol item of
         Some x \<Rightarrow> (
-          if doc!(bin s) = x then \<comment>\<open>Scan: x must then be a terminal\<close>
+          if doc!(bin s) = x then \<comment>\<open>Scan: x is a terminal\<close>
             let item' = inc_item item in
             State (update_bins (bins s) (bin s + 1) [item']) (bin s) (index s + 1)
-          else \<comment>\<open>Predict\<close>
-            undefined
+          else \<comment>\<open>Predict: x is a non-terminal\<close>
+            let rules' = filter (\<lambda>rule. rule_head rule = x) rules in
+            let items = map (\<lambda>rule. init_item rule (bin s)) rules' in
+            State (update_bins (bins s) (bin s) items) (bin s) (index s + 1)
         )
-      | None \<Rightarrow> undefined \<comment>\<open>Complete\<close>
+      | None \<Rightarrow> ( \<comment>\<open>Complete\<close>
+          let origin_bin = (bins s)!(item_origin item) in
+          let items = filter (\<lambda>item'. next_symbol item' = Some (item_rule_head item)) origin_bin in
+          let items' = map inc_item items in
+          State (update_bins (bins s) (bin s) items') (bin s) (index s + 1)
+        )
   )"
 
 function earley :: "state \<Rightarrow> state" where \<comment>\<open>TODO: Termination, REMARK: use while combinator\<close>
@@ -134,46 +155,33 @@ function earley :: "state \<Rightarrow> state" where \<comment>\<open>TODO: Term
 termination
   sorry
 
-definition earley_recognised :: "state \<Rightarrow> bool" where \<comment>\<open>TODO: call earley with inital state\<close>
-  "earley_recognised s \<longleftrightarrow> find is_finished ((bins s)!length doc) \<noteq> None"
+definition init_earley_state :: "state" where
+  "init_earley_state = (
+    let init_rules = filter (\<lambda>rule. rule_head rule = \<SS>) rules in
+    let init_items = map (\<lambda>rule. init_item rule 0) init_rules in
+    let bins = replicate (length doc + 1) [] in
+    State (update_bins bins 0 init_items) 0 0
+  )"
+
+definition earley_recognised :: "bool" where
+  "earley_recognised \<longleftrightarrow> (
+    let state = earley init_earley_state in
+    contains is_finished ((bins state)!length doc)
+  )"
+
+subsection \<open>Proofs\<close>
+
+lemma earley_step_fixpoint':
+  "earley_step (earley_step s) = s \<Longrightarrow> earley_step s = s"
+  unfolding earley_step_def is_finished_state_def
+  apply (auto simp: Let_def split!: option.splits if_splits)
+  apply (metis Suc_n_not_le_n n_not_Suc_n nat_le_linear le_SucI le_refl state.sel(2,3))+
+  done
+
+lemma earley_step_fixpoint:
+  "(earley_step s = s) \<longleftrightarrow> earley_step (earley_step s) = s"
+  using earley_step_fixpoint' by auto
 
 end
-
-context LocalLexing begin
-
-definition Predict :: "nat \<Rightarrow> items \<Rightarrow> items"
-where
-  "Predict k I = I \<union>  
-     { init_item r k | r x. r \<in> \<RR> \<and> x \<in> bin I k \<and> 
-       next_symbol x = Some(fst r) }"
-
-definition Complete :: "nat \<Rightarrow> items \<Rightarrow> items"
-where
-  "Complete k I = I \<union> { inc_item x k | x y. 
-     x \<in> bin I (item_origin y) \<and> y \<in> bin I k \<and> is_complete y \<and> 
-     next_symbol x = Some (item_nonterminal y) }"
-      
-definition \<pi> :: "nat \<Rightarrow> token set \<Rightarrow> items \<Rightarrow> items"
-where
-  "\<pi> k T I = 
-     limit (\<lambda> I. Scan T k (Complete k (Predict k I))) I"
-
-fun \<J> :: "nat \<Rightarrow> nat \<Rightarrow> items"
-and \<I> :: "nat \<Rightarrow> items"
-and \<T> :: "nat \<Rightarrow> nat \<Rightarrow> token set"
-where
-  "\<J> 0 0 = \<pi> 0 {} Init"
-| "\<J> k (Suc u) = \<pi> k (\<T> k (Suc u)) (\<J> k u)"
-| "\<J> (Suc k) 0 = \<pi> (Suc k) {} (\<I> k)"
-| "\<T> k 0 = {}"
-| "\<T> k (Suc u) = Tokens k (\<T> k u) (\<J> k u)"
-| "\<I> k = natUnion (\<J> k)"
-
-definition \<II> :: "items"
-where
-  "\<II> = \<I> (length Doc)"
-
-end
-
 
 end
